thy/Bitmagic/IPAddr.thy
@@ -1,0 +1,276 @@
+(*  Title:      IPAddr.thy
+    Authors:    Cornelius Diekmann
+*)
+theory IPAddr
+imports Main
+  NumberWang
+  WordInterval_Lists
+  "~~/src/HOL/Word/Word"
+  "./l4v/lib/WordLemmaBucket" (*will things break if I include this early?*)
+begin
+
+section {*Modelling IP Adresses*}
+  text{*An IP address is basically a unsigned integer.
+        We model IP addresses of arbitrary lengths.
+        The files @{file "IPv4Addr.thy"} @{file "IPv6Addr.thy"} concrete this for IPv4 and IPv6.*}
+
+  text{*The maximum IP addres*}
+  definition max_ip_addr :: "'i::len word" where 
+    "max_ip_addr \<equiv> of_nat ((2^(len_of(TYPE('i)))) - 1)"
+
+  lemma max_ip_addr_max_word: "max_ip_addr = max_word"
+    by(simp add: max_ip_addr_def max_word_def word_of_int_minus)
+    
+  lemma max_ipv4_addr_max: "\<forall>a. a \<le> max_ip_addr"
+    by(simp add: max_ip_addr_max_word)
+  lemma range_0_max_UNIV: "UNIV = {0 .. max_ip_addr}" (*not in the simp set, for a reason*)
+    by(simp add: max_ip_addr_max_word) fastforce
+
+  lemma size_ipaddr: "size (x::'i::len word) = len_of(TYPE('i))" by(simp add:word_size)
+
+  text{*previous and next IP addresses, without wrap around*}
+    definition ip_next :: "'i::len word \<Rightarrow> 'i word" where
+      "ip_next a \<equiv> if a = max_ip_addr then max_ip_addr else a + 1"
+    definition ip_prev :: "'i::len word \<Rightarrow> 'i word" where
+      "ip_prev a \<equiv> if a = 0 then 0 else a - 1"
+  
+    lemma "ip_next (2::8 word) = 3" by eval
+    lemma "ip_prev (2::8 word) = 1" by eval
+    lemma "ip_prev (0::8 word) = 0" by eval
+
+subsection{*Sets of IP addresses*}
+
+  (*Warning, not executable!*)
+  text{*192.168.0.0 255.255.255.0*}
+  definition ipset_from_netmask::"'i::len word \<Rightarrow> 'i::len word \<Rightarrow> 'i::len word set" where
+    "ipset_from_netmask addr netmask \<equiv> let network_prefix = (addr AND netmask) in {network_prefix .. network_prefix OR (NOT netmask)}"
+  (*Example: ipset_from_netmask 192.168.1.129  255.255.255.0  = {192.168.1.0 .. 192.168.1.255}*)
+
+  text{*192.168.0.0/24*}
+  definition ipset_from_cidr ::"'i::len word \<Rightarrow> nat \<Rightarrow> 'i::len word set" where
+    "ipset_from_cidr addr pflength \<equiv> ipset_from_netmask addr ((mask pflength) << (len_of(TYPE('i)) - pflength))"
+  (*Example: ipset_from_cidr 192.168.1.129 24  = {192.168.1.0 .. 192.168.1.255}*)
+
+  lemma ipset_from_cidr_0: "ipset_from_cidr foo 0 = UNIV"
+    by(auto simp add: ipset_from_cidr_def ipset_from_netmask_def Let_def)
+
+  
+  (*alternate definition*)
+  lemma ipset_from_cidr_alt1: fixes addr :: "'i::len word"
+    shows "ipset_from_cidr addr pflength = ipset_from_netmask addr ((mask pflength) << (len_of(TYPE('i)) - pflength))"
+    by(simp add: ipset_from_cidr_def)
+
+
+  lemma ipset_from_cidr_alt2:
+    fixes addr :: "'i::len word"
+    shows "ipset_from_cidr addr pflength \<equiv> 
+            ipset_from_netmask addr (of_bl ((replicate pflength True) @ (replicate ((len_of(TYPE('i))) - pflength)) False))"
+    by(simp add: ipset_from_cidr_alt1 mask_bl Word.shiftl_of_bl)
+
+
+  (*TODO: obsoletes NOT_mask_len32, requires WordLemmaBucket.*)
+  (*TODO: add to l4v*)
+  lemma NOT_mask_shifted_lenword: "NOT ((mask len << (len_of(TYPE('a)) - len))::'a::len word) = (mask (len_of(TYPE('a)) - len))"
+    apply(rule Word.word_bool_alg.compl_unique)
+     using WordLemmaBucket.mask_shift_and_negate apply(simp; fail)
+    apply (rule word_eqI)
+    apply (simp add: word_size nth_shiftl nth_shiftr)
+    apply auto
+    done
+
+  lemma ipset_from_cidr_alt: 
+    fixes pre :: "'i::len word"
+    shows "ipset_from_cidr pre len = {(pre AND ((mask len) << (len_of(TYPE('i)) - len))) .. pre OR (mask (len_of(TYPE('i)) - len))}"
+    apply(simp only: ipset_from_cidr_alt1 ipset_from_netmask_def Let_def)
+    apply(subst Word.word_oa_dist)
+    apply(simp only: word_or_not)
+    apply(simp only: Word.word_and_max)
+    apply(simp add: NOT_mask_shifted_lenword)
+    done
+
+  lemma "ipset_from_cidr 0 0 = UNIV" using ipset_from_cidr_0 by blast
+
+  lemma ipset_from_prefix_wordlength: 
+    fixes foo :: "'i::len word"
+    shows "ipset_from_cidr foo (len_of TYPE('i)) = {foo}"
+    by(simp add: ipset_from_cidr_alt1 ipset_from_netmask_def Let_def mask_def)
+
+
+(*
+  text{*making element check executable*}
+  lemma addr_in_ipv4range_set_from_netmask_code[code_unfold]: 
+    "addr \<in> (ipv4range_set_from_netmask base netmask) \<longleftrightarrow> (base AND netmask) \<le> addr \<and> addr \<le> (base AND netmask) OR (NOT netmask)"
+    by(simp add: ipv4range_set_from_netmask_def Let_def)
+  lemma addr_in_ipv4range_set_from_prefix_code[code_unfold]: "addr \<in> (ipv4range_set_from_prefix pre len) \<longleftrightarrow> 
+              (pre AND ((mask len) << (32 - len))) \<le> addr \<and> addr \<le> pre OR (mask (32 - len))"
+  unfolding ipv4range_set_from_prefix_alt by simp
+
+  value "ipv4addr_of_dotdecimal (192,168,4,8) \<in> (ipv4range_set_from_prefix (ipv4addr_of_dotdecimal (192,168,0,42)) 16)"
+
+  
+
+
+  definition ipv4range_single :: "ipv4addr \<Rightarrow> 32 wordinterval" where
+    "ipv4range_single ip \<equiv> WordInterval ip ip"
+
+  fun ipv4range_range :: "(ipv4addr \<times> ipv4addr) \<Rightarrow> 32 wordinterval" where
+    "ipv4range_range (ip_start, ip_end) = WordInterval ip_start ip_end"
+  declare ipv4range_range.simps[simp del]
+
+  definition ipv4range_to_set :: "32 wordinterval \<Rightarrow> (ipv4addr) set" where
+    "ipv4range_to_set rg = wordinterval_to_set rg"
+
+  definition ipv4range_element :: "'a::len word \<Rightarrow> 'a::len wordinterval \<Rightarrow> bool" where
+    "ipv4range_element el rg = wordinterval_element el rg"
+
+  definition ipv4range_union :: "32 wordinterval \<Rightarrow> 32 wordinterval \<Rightarrow> 32 wordinterval" where 
+    "ipv4range_union r1 r2 = wordinterval_union r1 r2"
+
+  definition ipv4range_empty :: "32 wordinterval \<Rightarrow> bool" where
+    "ipv4range_empty rg = wordinterval_empty rg"
+
+  definition ipv4range_setminus :: "32 wordinterval \<Rightarrow> 32 wordinterval \<Rightarrow> 32 wordinterval" where
+    "ipv4range_setminus r1 r2 = wordinterval_setminus r1 r2"
+
+  definition ipv4range_UNIV :: "32 wordinterval" where "ipv4range_UNIV \<equiv> wordinterval_UNIV"
+    
+  definition ipv4range_invert :: "32 wordinterval \<Rightarrow> 32 wordinterval" where 
+    "ipv4range_invert r = ipv4range_setminus ipv4range_UNIV r"
+
+  definition ipv4range_intersection :: "32 wordinterval \<Rightarrow> 32 wordinterval \<Rightarrow> 32 wordinterval" where
+    "ipv4range_intersection r1 r2 = wordinterval_intersection r1 r2"
+
+  definition ipv4range_subset:: "32 wordinterval \<Rightarrow> 32 wordinterval \<Rightarrow> bool" where
+    "ipv4range_subset r1 r2 \<equiv> wordinterval_subset r1 r2"
+
+  definition ipv4range_eq :: "32 wordinterval \<Rightarrow> 32 wordinterval \<Rightarrow> bool" where 
+    "ipv4range_eq r1 r2 = wordinterval_eq r1 r2"
+
+
+
+
+  lemma ipv4range_single_set_eq: "ipv4range_to_set (ipv4range_single ip) = {ip}"
+    by(simp add: ipv4range_single_def ipv4range_to_set_def)
+  lemma ipv4range_range_set_eq: "ipv4range_to_set (ipv4range_range (ip1, ip2)) = {ip1 .. ip2}"
+    by(simp add: ipv4range_range.simps ipv4range_to_set_def)
+  
+  lemma ipv4range_element_set_eq[simp]: "ipv4range_element el rg = (el \<in> ipv4range_to_set rg)"
+    by(simp add: ipv4range_element_def ipv4range_to_set_def)
+  lemma ipv4range_union_set_eq[simp]: "ipv4range_to_set (ipv4range_union r1 r2) = ipv4range_to_set r1 \<union> ipv4range_to_set r2"
+    by(simp add: ipv4range_to_set_def ipv4range_union_def)
+  lemma ipv4range_empty_set_eq[simp]: "ipv4range_empty r \<longleftrightarrow> ipv4range_to_set r = {}"
+    by(simp add: ipv4range_to_set_def ipv4range_empty_def)
+  lemma ipv4range_setminus_set_eq[simp]: "ipv4range_to_set (ipv4range_setminus r1 r2) = ipv4range_to_set r1 - ipv4range_to_set r2"
+    by(simp add: ipv4range_setminus_def ipv4range_to_set_def)
+  lemma ipv4range_UNIV_set_eq[simp]: "ipv4range_to_set ipv4range_UNIV = UNIV"
+    by(simp only: ipv4range_UNIV_def ipv4range_to_set_def wordinterval_UNIV_set_eq)
+  lemma ipv4range_invert_set_eq[simp]: "ipv4range_to_set (ipv4range_invert r) = UNIV - ipv4range_to_set r"
+    by(simp add: ipv4range_invert_def)
+  lemma ipv4range_intersection_set_eq[simp]: "ipv4range_to_set (ipv4range_intersection r1 r2) = ipv4range_to_set r1 \<inter> ipv4range_to_set r2"
+    by(simp add: ipv4range_intersection_def ipv4range_to_set_def)
+  lemma ipv4range_subset_set_eq[simp]: "ipv4range_subset r1 r2 = (ipv4range_to_set r1 \<subseteq> ipv4range_to_set r2)"
+    by(simp add: ipv4range_subset_def ipv4range_to_set_def)
+  lemma ipv4range_eq_set_eq: "ipv4range_eq r1 r2 \<longleftrightarrow> ipv4range_to_set r1 = ipv4range_to_set r2"
+    unfolding ipv4range_eq_def ipv4range_to_set_def using wordinterval_eq_set_eq by blast
+
+  declare ipv4range_range_set_eq[unfolded ipv4range_range.simps, simp]
+  declare ipv4range_union_set_eq[unfolded ipv4range_union_def wordinterval_union_def, simp]
+
+
+  thm iffD1[OF ipv4range_eq_set_eq]
+  declare iffD1[OF ipv4range_eq_set_eq, cong]
+  lemma ipv4range_eq_comm: "ipv4range_eq r1 r2 \<longleftrightarrow> ipv4range_eq r2 r1"
+    unfolding ipv4range_eq_def wordinterval_eq_set_eq by blast
+  lemma ipv4range_to_set_alt: "ipv4range_to_set r = {x. ipv4range_element x r}"
+    unfolding ipv4range_element_set_eq by blast
+ 
+  lemma ipv4range_un_empty: "ipv4range_empty r1 \<Longrightarrow> ipv4range_eq (ipv4range_union r1 r2) r2"
+    by(subst ipv4range_eq_set_eq, simp)
+  lemma ipv4range_un_emty_b: "ipv4range_empty r2 \<Longrightarrow> ipv4range_eq (ipv4range_union r1 r2) r1"
+    by(subst ipv4range_eq_set_eq, simp)
+  
+  lemma ipv4range_Diff_triv: "ipv4range_empty (ipv4range_intersection a b) \<Longrightarrow> ipv4range_eq (ipv4range_setminus a b) a"
+    unfolding ipv4range_eq_set_eq by(simp add: Diff_triv )
+    (*by(simp only: wordinterval_Diff_triv ipv4range_eq_def ipv4range_setminus_def ipv4range_intersection_def wordinterval_intersection_def ipv4range_empty_def)*)
+
+
+  lemma 
+  	fixes k :: "'a :: complete_lattice"
+  	shows "is_lowest_element x S \<longleftrightarrow> (x::'a) = Inf S"
+  oops (*Auto Quickcheck found a counterexample:*)
+    
+  fun ipv4range_lowest_element :: "32 wordinterval \<Rightarrow> ipv4addr option" where
+    "ipv4range_lowest_element (WordInterval s e) = (if s \<le> e then Some s else None)" | 
+    "ipv4range_lowest_element (RangeUnion A B) = (case (ipv4range_lowest_element A, ipv4range_lowest_element B) of
+      (Some a, Some b) \<Rightarrow> Some (if a < b then a else b) |
+      (None, Some b) \<Rightarrow> Some b |
+      (Some a, None) \<Rightarrow> Some a |
+      (None, None) \<Rightarrow> None)"
+
+  lemma ipv4range_lowest_none_empty: "ipv4range_lowest_element r = None \<longleftrightarrow> ipv4range_empty r"
+    proof(induction r)
+    case WordInterval thus ?case by simp
+    next
+    case RangeUnion thus ?case by fastforce
+    qed
+    
+
+  lemma ipv4range_lowest_element_correct_A: "ipv4range_lowest_element r = Some x \<Longrightarrow> is_lowest_element x (ipv4range_to_set r)"
+    unfolding is_lowest_element_def
+    apply(induction r arbitrary: x rule: ipv4range_lowest_element.induct)
+     apply(rename_tac rs re x, case_tac "rs \<le> re", auto)[1]
+    apply(subst(asm) ipv4range_lowest_element.simps(2))
+    apply(rename_tac A B x)
+    apply(case_tac     "ipv4range_lowest_element B")
+     apply(case_tac[!] "ipv4range_lowest_element A")
+       apply(simp_all add: ipv4range_lowest_none_empty)[3]
+    apply fastforce
+  done
+
+
+  lemma ipv4range_lowest_element_set_eq: assumes "\<not> ipv4range_empty r"
+    shows "(ipv4range_lowest_element r = Some x) = (is_lowest_element x (ipv4range_to_set r))"
+    (*unfolding is_lowest_element_def*)
+    proof(rule iffI)
+      assume "ipv4range_lowest_element r = Some x"
+      thus "is_lowest_element x (ipv4range_to_set r)"
+     using ipv4range_lowest_element_correct_A ipv4range_lowest_none_empty by simp
+    next
+      assume "is_lowest_element x (ipv4range_to_set r)"
+      with assms show "(ipv4range_lowest_element r = Some x)"
+        proof(induction r arbitrary: x rule: ipv4range_lowest_element.induct)
+        case 1 thus ?case by(simp add: is_lowest_element_def)
+        next
+        case (2 A B x)
+
+        have is_lowest_RangeUnion: "is_lowest_element x (ipv4range_to_set A \<union> ipv4range_to_set B) \<Longrightarrow> 
+          is_lowest_element x (ipv4range_to_set A) \<or> is_lowest_element x (ipv4range_to_set B)"
+          by(simp add: is_lowest_element_def)
+      
+         (*why \<And> A B?*)
+         have ipv4range_lowest_element_RangeUnion: "\<And>a b A B. ipv4range_lowest_element A = Some a \<Longrightarrow> ipv4range_lowest_element B = Some b \<Longrightarrow>
+                  ipv4range_lowest_element (RangeUnion A B) = Some (min a b)"
+           by(auto dest!: ipv4range_lowest_element_correct_A simp add: is_lowest_element_def min_def)
+         
+        from 2 show ?case
+        apply(case_tac     "ipv4range_lowest_element B")
+         apply(case_tac[!] "ipv4range_lowest_element A")
+           apply(auto simp add: is_lowest_element_def)[3]
+        apply(subgoal_tac "\<not> ipv4range_empty A \<and> \<not> ipv4range_empty B")
+         prefer 2
+         using arg_cong[where f = Not, OF ipv4range_lowest_none_empty] apply(simp, metis)
+        apply(drule(1) ipv4range_lowest_element_RangeUnion)
+        apply(simp split: option.split_asm add: min_def)
+         apply(drule is_lowest_RangeUnion)
+         apply(elim disjE)
+          apply(simp add: is_lowest_element_def)
+         apply(clarsimp simp add: ipv4range_lowest_none_empty)
+        
+        apply(simp add: is_lowest_element_def)
+        apply(clarsimp simp add: ipv4range_lowest_none_empty)
+        using ipv4range_lowest_element_correct_A[simplified is_lowest_element_def]
+        by (metis Un_iff not_le)
+      qed
+    qed
+*)
+end
