thy/Bitmagic/IPv4Addr.thy
@@ -384,7 +384,7 @@ subsection{*IP ranges*}
   lemma 
   	fixes k :: "'a :: complete_lattice"
   	shows "is_lowest_element x S \<longleftrightarrow> (x::'a) = Inf S"
-  oops
+  oops (*Auto Quickcheck found a counterexample:*)
     
   fun ipv4range_lowest_element :: "32 wordinterval \<Rightarrow> ipv4addr option" where
     "ipv4range_lowest_element (WordInterval s e) = (if s \<le> e then Some s else None)" | 
